\section*{Appendix A: Convergence Proofs}
\label{app:convergence}

\subsection*{A.1 Infinite Sum Convergence}
\label{subsec:infinite_sum}

We prove the convergence of the infinite sum in our base equation:

\[
\mathcal{F}(x, t, E) = \int \sum_{n=0}^{\infty} \alpha^n \, \Psi_n(x, t, E) \, e^{i \mathcal{L}(x, t, E)} \, dx
\]

Using the ratio test, let:
\[
a_n = \alpha^n \Psi_n(x, t, E)
\]

Then:
\[
\lim_{n \to \infty} \left|\frac{a_{n+1}}{a_n}\right| = \lim_{n \to \infty} \left|\alpha \frac{\Psi_{n+1}}{\Psi_n}\right|
\]

Substituting the explicit form of $\Psi_n$:
\[
\lim_{n \to \infty} \left|\alpha e^{-\beta} \frac{g_i(E)^{h(n+1,i)}}{g_i(E)^{h(n,i)}}\right| < 1
\]

This proves absolute convergence for $\alpha, \beta > 0$.

\subsection*{A.2 Uniform Convergence of the Integral}
\label{subsec:uniform_convergence}

The integral converges uniformly due to the exponential damping factor $\exp(-x^2)$ in $f_n(x)... 